refractoring : moved things to right places. cleaned and fully compiled (using scons) src/ and examples/icreateMoveToLoc/ As usual, some Coq files failed to compile. As usual, they are not in use anymore. Removed them from the SConstruct

src/StdlibMisc.v
@@ -285,3 +285,6 @@ Proof.
     assert (c = b ∨ c < b) as Hd by omega.
     destruct Hd; try congruence.
 Qed.
+
+Inductive Truncate (T:Type) : Prop :=
+| truncate : T -> Truncate T.
